Intermediate

theories/metaconfig.v
@@ -2,6 +2,7 @@ Require Import List.
 Import ListNotations.
 From stdpp Require Import base gmap.
 From Coq Require Import String.
+Require Import Coq.Classes.DecidableClass.
 
 (** Represent the registers of a process as a map between identifiers and their integer value *)
 (* Definition register_file := gmap string nat. *)
@@ -20,14 +21,28 @@ Variant register (Name : Type) : Type :=
   }.
 End RegisterFile. *)
 
-Record object_type (Π : Type) := {
+Record object_type (Value Π : Type) := {
   Σ : Type;
   OP : Type;
-  ARG : OP → Type;
-  RES : Type;
-  δ : Σ → Π → ∀ (op : OP), ARG op → Σ * RES;
+  ARG : OP → Value → Prop;
+  RES : Value → Prop;
+  δ : Σ → Π → ∀ op, { v | ARG op v } → Σ * { v | RES v };
 }.
 
+Definition states {Value Π : Type} (ty : object_type Value Π) :=
+  ty.(Σ Value Π).
+
+Definition operations {Value Π : Type} (ty : object_type Value Π) :=
+  ty.(OP Value Π).
+
+Definition arguments {Value Π : Type} (ty : object_type Value Π) op :=
+  { v | ty.(ARG Value Π) op v }.
+
+Definition results  {Value Π : Type} (ty : object_type Value Π) :=
+  { v | ty.(RES Value Π) v }.
+
+
+(* 
 Module Queue.
 
   Variant op : Set := Enqueue | Dequeue.
@@ -80,7 +95,7 @@ Module Queue.
              end;
     |}.
 
-End Queue.
+End Queue. *)
 
 (* Record object (Π : Type) := {
   type : object_type Π;
@@ -92,8 +107,8 @@ End Queue.
    and also make modifications to its private registers.
    So, represent program as a relation relating *)
 
-Class Object (Ω : Type) (Π : Type) := {
-  type : Ω → object_type Π;
+Class Object (Value : Type) (Π : Type) (Ω : Type) := {
+  type : Ω → object_type Value Π;
   (* state : ∀ (ω : Ω), (type ω).(Σ Π) *)
 }.
 
@@ -107,72 +122,134 @@ Class Process (Π : Type) := {
   base_objects : Type;
 }. *)
 
-Inductive value :=
-  | Int (n : Z)
-  | Bool (b : bool)
-  | Unit.
+(* 
+Class EqDec (A : Type) :=
+  { eqb : A → A → bool ;
+    eqb_leibniz x y : eqb x y = true → x = y }.
+    
+Lemma z_eqb_leibniz x y : Z.eqb x y = true → x = y.
+Proof.
+  intros.
+  apply Z.eqb_eq.
+  assumption.
+Defined.
+
+Instance Z_EqDec : EqDec Z := {
+  eqb := Z.eqb;
+  eqb_leibniz := z_eqb_leibniz;
+}.
+
+Lemma bool_eqb_leibniz x y : Bool.eqb x y = true → x = y.
+Proof.
+  intros.
+  apply Bool.eqb_eq.
+  auto.
+Defined.
+
+Instance bool_EqDec : EqDec bool := {
+  eqb := Bool.eqb;
+  eqb_leibniz := bool_eqb_leibniz;
+}.
+
+Definition eqb_unit (tt : unit) (tt : unit) := true.
+
+Lemma unit_eqb_leibniz x y : eqb_unit x y = true → x = y.
+Proof.
+  destruct x, y. trivial.
+Defined. 
+
+Instance unit_EqDec : EqDec unit := {
+  eqb := eqb_unit;
+  eqb_leibniz := unit_eqb_leibniz;
+}.
+
+Definition eqb_value v v' :=
+  match v, v' with
+  | Int n, Int n' => eqb n n'
+  | Bool b, Bool b' => eqb b b'
+  | Unit, Unit => true
+  | _, _ => false
+  end.
+
+Theorem value_eqb_leibniz v v' : eqb_value v v' = true → v = v'.
+Proof.
+  intros. destruct v, v'; simpl in *; try discriminate.
+  - apply z_eqb_leibniz in H. congruence.
+  - apply bool_eqb_leibniz in H. congruence.
+  - reflexivity.
+Defined.
+
+Instance value_EqDec : EqDec value := {
+  eqb := eqb_value;
+  eqb_leibniz := value_eqb_leibniz;
+}. *)
+
+Definition register_assignment {Π : Type} `{Process Π} (π : Π) (Value : Type) :=
+  register_names π → Value.
 
 Section Run.
 
-  Variables Ω Π : Type.
+  Variable Value : Type.
 
-  Context `{Object Ω Π} `{Process Π}.
+  Variable Π : Type.
 
-  Record configuration := {
+  Context `{Process Π}.
+
+  Record configuration (Ω : Type) `{Object Value Π Ω} := {
     (* Private registers of each process *)
-    register_values (π : Π) : register_names π → value;
+    register_values π : register_assignment π Value;
     (* Program counter of each process *)
     pc : Π → nat;
+    (* Return value register of each process *)
+    (* ret : Π → Value; *)
     (* Assignment of state to every object *)
-    object_states (ω : Ω) : (type ω).(Σ Π);
+    object_states (ω : Ω) : (type ω).(Σ Value Π);
   }.
 
+  Variable Ω : Type.
+
+  Context `{Object Value Π Ω}.
+
+  Definition sem := configuration Ω → Π → nat → configuration Ω → Prop.
+
   (* Describes semantics of program *)
-  Variable step : configuration → Π → nat → configuration → Prop.
+  Variable step : configuration Ω → Π → nat → configuration Ω → Prop.
 
   (** Well-formedness condition requiring that one process taking 
       a step doesn't affect the private registers of other processes *)
-  Variable step_wf : 
-    ∀ c π π' l c',
+  Inductive Step_wf : Prop :=
+    Step_wf_intro c π π' l c' :
       (* If (c, (π, l), c') is a step *)
       step c π l c' →
-      (* For any other process π' *)
+      (* program counter of π is at l *)
+      pc Ω c π = l /\
+      (* And, for any other process π' *)
       π <> π' →
-      (* The private registers of π are the same in c' as in c *)
-      register_values c π' = register_values c' π'.
+      (* The private registers of π' are the same in c' as in c *)
+      register_values Ω c π' = register_values Ω c' π'
+      → Step_wf.
 
   CoInductive run : Type :=
-    | Final (final : configuration)
-    | Step (π : Π) (l : nat) (conf : configuration) (tl : run).
+    | Final (c : configuration Ω)
+    | Step (c : configuration Ω) (π : Π) (l : nat) (tl : run).
 
-  CoInductive run' : Type :=
-    | Nil
-    | Cons (π : Π) (l : nat) (conf : configuration) (tl : run').
+  Inductive Finite : run → Prop :=
+    | FiniteFinal c : Finite (Final c)
+    | FiniteStep c π l tl : Finite tl → Finite (Step c π l tl).
 
-  CoInductive Run' (c : configuration) : run' → Prop :=
-    | RunNil : Run' c Nil
-    | RunCons π l c' tl : step c π l c' → Run' c' tl → Run' c (Cons π l c' tl).
+  CoInductive Infinite : run → Prop := 
+    Infinite_intro c π l tl : Infinite tl → Infinite (Step c π l tl).
 
-  Inductive Finite' : run' → Prop :=
-    | FiniteNil : Finite' Nil
-    | FiniteCons π l conf tl : Finite' tl → Finite' (Cons π l conf tl).
+  Definition initial_config r :=
+    match r with
+    | Final c | Step c _ _ _ => c
+    end.
 
-  CoInductive Infinite' : run' → Prop :=
-    Infinite_intro' π l conf tl : Infinite' tl → Infinite' (Cons π l conf tl).
+  CoInductive Run : run → Prop :=
+    | RunFinal c : Run (Final c)
+    | RunStep c π l tl : step c π l (initial_config tl) → Run tl → Run (Step c π l tl).
 
-  Variant run : Type := Run (initial : configuration) (tl : run').
-
-  Variant Is_run : run → Prop :=
-    Is_run_intro initial tl : Run' initial tl → Is_run (Run initial tl).
-
-  Variant Finite : run → Prop :=
-    Finite_intro initial tl : Finite' tl → Finite (Run initial tl).
-
-  
-
-   
-
-  (* Inductive run : Type :=
+(* Inductive run : Type :=
     | Initial (initial : configuration)
     | Step (prefix : run) (π : Π) (l : nat) (conf : configuration).
     
@@ -187,9 +264,69 @@ Section Run.
     | RunStep (prefix : run) (π : Π) (l : nat) (c : configuration) : 
         Run prefix → step (final_configuration prefix) π l c → Run (Step prefix π l c). *)
 
+  (* A program is list of program lines describing the changes in state from line to line *)
+
 End Run.
 
-Check EqDec.
+
+Section Implementation.
+
+  Variable Π : Type.
+
+  Context `{Process Π}.
+
+  Variable Ω : Type.
+
+  Context `{Object Value Π Ω}.
+
+  (** Base objects *)
+  Variable Ψ : Type.
+
+  Context `{Object Value Π Ψ}.
+
+  Variable ω : Ω.
+
+  Record Invocation := {
+    ψ : Ψ;
+    op : operations (type ψ);
+    arg : arguments (type ψ) op;
+  }.
+
+  (* Inductive line (π : Π) : Type :=
+    Line 
+      (invs : list Invocation) (* Invocations on base objects possibly performed *)
+      (transition : 
+        { results | Forall2 (fun inv => (type (inv.(ψ))).(RES Value Π)) invs results } → (* Results from operations on base objects *)
+        nat (* Current program counter *) →
+        register_assignment π Value → (* And current value of private registers *)
+        nat * register_assignment π Value (* Compute next PC and values of private registers *)). *)
+
+    Inductive line (π : Π) : Type :=
+      | Write (register_assignment π → Value) (r : register_names π).
+      (* Line 
+        (invs : list Invocation) (* Invocations on base objects possibly performed *)
+        (transition : 
+          { results | Forall2 (fun inv => (type (inv.(ψ))).(RES Value Π)) invs results } → (* Results from operations on base objects *)
+          nat (* Current program counter *) →
+          register_assignment π Value → (* And current value of private registers *)
+          nat * register_assignment π Value (* Compute next PC and values of private registers *)). *)
+
+
+  Record procedure (π : Π) (op : operations (type ω)) (arg : arguments (type ω) op) := {
+    ret : register_names π;
+    lines : list (line π);
+  }.
+
+  (* Implementation of [ω ∈ Ω] using objects from [Ψ]] *)
+  Record Implementation := 
+  {
+    inital_states (ψ : Ψ) : states (type ψ);
+    procedures π op arg : procedure π op arg;
+  }. 
+
+End Implementation.
+
+End Metaconfig.
 
 (* Module Objects.
   Record t (Π : Type) := {
@@ -205,7 +342,7 @@ End Objects. *)
   }.
 End Processes. *)
 
-Record configuration (Ω : Type) (Π : Type) (object_types : Ω → object_type Π) (registers : Π → Type) := {
+(* Record configuration (Ω : Type) (Π : Type) (object_types : Ω → object_type Π) (registers : Π → Type) := {
   (* Assignment of state to every object *)
   object_states : ∀ (ω : Ω), (object_types ω).(Σ Π);
   (* Assignment of values to every private register *)
@@ -347,4 +484,4 @@ Proof.
   admit.
 Admitted.
 
-End Metaconfig.
+End Metaconfig. *)
