theories/Dynamics.v
@@ -1,0 +1,13 @@
+Require Import Metaconfigurations.Syntax.
+
+(** Machine configurations are represented as tuples [⟨ σ , ϵ , e ⟩] where [σ] 
+    binds thread-local variables to their values, [δ] binds object names to object states,
+    ϵ binds object names to object types, and [e] is a term *)
+Reserved Notation "⟨ σ , δ , ϵ , e ⟩ ⇓ v"
+         (at level 80, no associativity).
+
+Module Expr.
+  (* configuration should include store bindings from thread-local variables to values *)
+  Inductive Step : Type :=
+    | 
+End Expr.
