theories/Object.v
@@ -1,0 +1,17 @@
+From stdpp Require Import base gmap.
+Require Import Coq.Sets.Ensembles.
+Require Import Coq.Strings.String.
+From Metaconfigurations.Syntax Require Import Value Ty.
+From Metaconfigurations.Statics Require Import Value.
+
+Record object_type := {
+  Σ : Type;
+  OP : Type;
+  ARG : OP → Ty.t;
+  RES : OP → Ty.t;
+  δ : Σ → ∀ op, V⟦ ARG op ⟧ → V⟦ RES op ⟧;
+}.
+
+Class Object (Ω : Type) := {
+  type : Ω → object_type;
+}.
