theories/Statics/Value.v
@@ -1,0 +1,12 @@
+From stdpp Require Import base.
+Require Import Metaconfigurations.Syntax.Value.
+
+Inductive type : t → Ty.t → Prop :=
+  | type_int n : type (Int n) Ty.Int
+  | type_bool b : type (Bool b) Ty.Bool
+  | type_unit : type Unit Ty.Unit
+  | type_tuple vs τs : Forall2 type vs τs → type (Tuple vs) (Ty.Tuple τs).
+
+Definition with_type τ := { v | type v τ }.
+
+Notation "V⟦ τ ⟧" := (with_type τ).
