theories/Syntax/Term.v
@@ -1,0 +1,99 @@
+From stdpp Require Import base gmap.
+Require Import Coq.Strings.String.
+Require Import Coq.Lists.List.
+
+Module Expr.
+
+  Parameter Ω : Type.
+
+  Variant bop : Set :=
+    | Add
+    | Sub
+    | Mul
+    | And
+    | Or.
+
+  Variant uop : Set := Not.
+
+  Inductive t : Type :=
+    | Var (x : string)
+    | Call (obj : string) (op : string) (es : list t)
+    | Bop (op : bop) (e₁ : t) (e₂ : t)
+    | Uop (op : uop) (e : t)
+    | Tuple (es : list t)
+    | Int (n : Z)
+    | Bool (b : bool)
+    | Unit.
+
+  Section custom_ind.
+    Variable P : t → Prop.
+    Hypothesis HVar : ∀ x, P (Var x).
+    Hypothesis HCall : ∀ obj op es, Forall P es → P (Call obj op es).
+    Hypothesis HBop : ∀ op e₁ e₂, P e₁ → P e₂ → P (Bop op e₁ e₂).
+    Hypothesis HUop : ∀ op e, P e → P (Uop op e).
+    Hypothesis HTuple : ∀ es, Forall P es → P (Tuple es).
+    Hypothesis HInt : ∀ n, P (Int n).
+    Hypothesis HBool : ∀ b, P (Bool b).
+    Hypothesis HUnit : P Unit.
+
+    Definition custom_ind : ∀ e, P e :=
+      fix f e : P e :=
+        let flist (es : list t) : Forall P es :=
+          list_ind
+            (Forall P) (Forall_nil P)
+            (fun e l H => Forall_cons P e l (f e) H) es
+        in      
+        match e with
+        | Var x => HVar x
+        | Call obj op es => HCall obj op es (flist es)
+        | Bop op e₁ e₂ => HBop op e₁ e₂ (f e₁) (f e₂)
+        | Uop op e => HUop op e (f e)
+        | Tuple es => HTuple es (flist es)
+        | Int n => HInt n
+        | Bool b => HBool b
+        | Unit => HUnit
+        end.
+  End custom_ind.
+
+  Inductive Value : t → Prop :=
+    | ValueInt n : Value (Int n)
+    | ValueBool b : Value (Bool b)
+    | ValueUnit : Value Unit
+    | ValueTuple es : Forall Value es → Value (Tuple es).
+
+  Section custom_value_ind.
+    Variable P : t → Prop.
+    Hypothesis HInt : ∀ n, P (Int n).
+    Hypothesis HBool : ∀ b, P (Bool b).
+    Hypothesis HUnit : P Unit.
+    Hypothesis HTuple : ∀ vs, Forall Value vs → Forall P vs → P (Tuple vs).
+
+    Definition custom_value_ind : ∀ v, Value v → P v :=
+      fix f v H :=
+        match H with
+        | ValueInt n => HInt n
+        | ValueBool b => HBool b
+        | ValueUnit => HUnit
+        | ValueTuple vs Hvs =>
+          HTuple vs Hvs
+              (Forall_ind
+                    (Forall P)
+                    (Forall_nil P)
+                    (fun (v : t) (l : list t) (Hv : Value v) Hvs Hl => @Forall_cons t P v l (f v Hv) Hl) Hvs)
+        end.
+  End custom_value_ind.
+
+End Expr.
+
+Module Stmt.
+  Inductive t : Type :=
+    | Seq (s₁ : t) (s₂ : t)
+    | Assign (x : string) (e : Expr.t)
+    | If (e : Expr.t) (s₁ : t) (s₂ : t)
+    (* | While (e : Expr.t) (s : t) *)
+    | Goto (l : nat)
+    | Return (e : Expr.t)
+    | Call (obj : string) (op : string) (es : list t).
+End Stmt.
+
+
