theories/Syntax/Ty.v
@@ -1,0 +1,30 @@
+From stdpp Require Import base gmap.
+Require Import Coq.Lists.List.
+
+Inductive t : Type := 
+  | Int 
+  | Bool 
+  | Unit
+  | Tuple (τs : list t).
+
+Section custom_ind.
+  Variable P : t → Prop.
+
+  Hypothesis HInt : P Int.
+  Hypothesis HBool : P Bool.
+  Hypothesis HUnit : P Unit.
+  Hypothesis HTuple : ∀ τs, Forall P τs → P (Tuple τs).
+
+  Definition custom_ind : ∀ τ, P τ :=
+    fix f τ : P τ :=
+      match τ with
+      | Int => HInt
+      | Bool => HBool
+      | Unit => HUnit
+      | Tuple τs =>
+        HTuple τs
+          (list_ind
+              (Forall P) (Forall_nil P)
+              (fun τ l H => Forall_cons P τ l (f τ) H) τs)
+      end.
+End custom_ind.
