theories/Syntax/Value.v
@@ -1,0 +1,30 @@
+From stdpp Require Import base gmap.
+Require Import Metaconfigurations.Syntax.Ty.
+
+Inductive t :=
+  | Int (n : Z)
+  | Bool (b : bool)
+  | Unit
+  | Tuple (vs : list t).
+
+Section custom_ind.
+    Variable P : t → Prop.
+    Hypothesis HInt : ∀ n, P (Int n).
+    Hypothesis HBool : ∀ b, P (Bool b).
+    Hypothesis HUnit : P Unit.
+    Hypothesis HTuple : ∀ vs, Forall Value vs → Forall P vs → P (Tuple vs).
+
+    Definition custom_ind : ∀ v, Value v → P v :=
+      fix f v H :=
+        match H with
+        | ValueInt n => HInt n
+        | ValueBool b => HBool b
+        | ValueUnit => HUnit
+        | ValueTuple vs Hvs =>
+          HTuple vs Hvs
+              (Forall_ind
+                    (Forall P)
+                    (Forall_nil P)
+                    (fun (v : t) (l : list t) (Hv : Value v) Hvs Hl => @Forall_cons t P v l (f v Hv) Hl) Hvs)
+        end.
+  End custom_ind.
